src/dvc_implementation/dvc_externs.dfy
@@ -1,0 +1,160 @@
+include "../common/commons.dfy"
+
+module DVC_Externs
+{
+    import opened Types
+    import opened CommonFunctions
+
+    trait 
+    // See https://github.com/dafny-lang/dafny/issues/1588 for why {:termination false} is needed
+    {:termination false} 
+    {:autocontracts} ConsensusValidityCheck<T, SlashingDBType(==)>
+    {
+        const slashing_db: SlashingDB<SlashingDBType>
+
+        method is_valid(data: T) returns (validity: bool)
+    }    
+
+    trait {:autocontracts} Consensus<T(!new, ==), SlashingDBType(!new, ==)>
+    {
+        ghost var consensus_instances_started: map<Slot, ConsensusValidityCheck<T, SlashingDBType>>
+
+        method start(
+            id: Slot,
+            validityPredicate: ConsensusValidityCheck<T, SlashingDBType>
+        ) returns (s: Status)
+        ensures s.Success? <==> id !in old(consensus_instances_started.Keys)
+        ensures s.Success? ==> consensus_instances_started == old(consensus_instances_started)[id := validityPredicate]
+        ensures s.Failure? ==> unchanged(`consensus_instances_started)  
+
+        method stop_multiple(
+            ids: set<Slot>
+        )
+        ensures consensus_instances_started == old(consensus_instances_started) - ids
+
+        method get_active_instances() returns (active_instances: set<Slot>)
+        ensures active_instances == consensus_instances_started.Keys 
+        ensures unchanged(`consensus_instances_started) 
+    }    
+
+    trait {:autocontracts} Network  
+    {
+        ghost var att_shares_sent: seq<set<MessaageWithRecipient<AttestationShare>>>;
+
+        method send_att_share(att_share: AttestationShare, receipients: set<BLSPubkey>)
+        ensures att_shares_sent == old(att_shares_sent)  + [addRecepientsToMessage(att_share, receipients)]
+
+        method send_att_shares(att_shares: set<AttestationShare>, receipients: set<BLSPubkey>)
+        ensures     var setWithRecipient := set att_share | att_share in att_shares :: addRecepientsToMessage(att_share, receipients);
+                    att_shares_sent == old(att_shares_sent)  + [setUnion(setWithRecipient)]
+        ensures unchanged(`att_shares_sent)
+
+        ghost var sent_block_shares: seq<set<MessaageWithRecipient<SignedBeaconBlock>>>;
+        ghost var sent_randao_shares: seq<set<MessaageWithRecipient<RandaoShare>>>;
+
+        method send_block_share(block_share: SignedBeaconBlock, receipients: set<BLSPubkey>)
+        ensures sent_block_shares == old(sent_block_shares)  + [addRecepientsToMessage(block_share, receipients)]  
+        ensures unchanged(`sent_randao_shares)
+
+        method send_block_shares(block_shares: set<SignedBeaconBlock>, receipients: set<BLSPubkey>)
+        ensures var setWithRecipient := set block_share | block_share in block_shares :: addRecepientsToMessage(block_share, receipients);
+                sent_block_shares == old(sent_block_shares)  + [setUnion(setWithRecipient)]
+        ensures unchanged(`sent_randao_shares)        
+
+        method send_randao_share(randao_share: RandaoShare, receipients: set<BLSPubkey>)
+        ensures sent_randao_shares == old(sent_randao_shares)  + [addRecepientsToMessage(randao_share, receipients)]
+        ensures unchanged(`sent_block_shares)
+
+        method send_randao_shares(randao_shares: set<RandaoShare>, receipients: set<BLSPubkey>)
+        ensures var setWithRecipient := set randao_share | randao_share in randao_shares :: addRecepientsToMessage(randao_share, receipients);
+                sent_randao_shares == old(sent_randao_shares)  + [setUnion(setWithRecipient)]
+        ensures unchanged(`sent_block_shares)      
+
+    }
+
+    trait {:autocontracts} BeaconNode<T(!new, ==)>
+    {
+        ghost var state_roots_of_imported_blocks: set<Root>;
+        ghost var data_submitted: seq<T>; 
+
+        method get_fork_version(s: Slot) returns (v: Version)
+        ensures unchanged(`state_roots_of_imported_blocks)
+        ensures unchanged(`data_submitted)
+
+        method submit_data(data: T)
+        ensures data_submitted == old(data_submitted) + [data]
+        ensures unchanged(`state_roots_of_imported_blocks)
+
+        // https://ethereum.github.io/beacon-APIs/?urls.primaryName=v1#/Beacon/getEpochCommittees
+        method get_epoch_committees(
+            state_id: Root,
+            index: CommitteeIndex
+        ) returns (s: Status, sv: seq<ValidatorIndex>)
+        ensures unchanged(`state_roots_of_imported_blocks)
+        ensures unchanged(`data_submitted)        
+        ensures state_id in state_roots_of_imported_blocks <==> s.Success?
+        ensures uniqueSeq(sv)  
+
+        // https://ethereum.github.io/beacon-APIs/#/Beacon/getStateValidator
+        method get_validator_index(
+            state_id: Root,
+            validator_id: BLSPubkey
+        ) returns (s: Status, vi: Optional<ValidatorIndex>)
+        ensures unchanged(`state_roots_of_imported_blocks)
+        ensures unchanged(`data_submitted)        
+        ensures state_id in state_roots_of_imported_blocks <==> s.Success?
+    }
+
+    trait {:autocontracts} RemoteSigner
+    {
+        const pubkey: BLSPubkey;
+
+        method sign_attestation(
+            attestation_data: AttestationData, 
+            fork_version: Version, 
+            signing_root: Root           
+        ) returns (s: BLSSignature)
+        requires signing_root == compute_attestation_signing_root(attestation_data, fork_version)
+
+        // eth_node_interface.py --> rs_sign_block
+        method sign_block(
+            block: BeaconBlock,
+            fork_version: Version, 
+            signing_root: Root           
+        ) returns (s: BLSSignature)
+        requires signing_root == compute_block_signing_root(block)
+
+        // eth_node_interface.py --> rs_sign_randao_reveal
+        // Check the pre-condition that is based on the first slot of an epoch.
+        method {:extern} sign_randao_reveal(
+            epoch: Epoch,
+            fork_version: Version, 
+            signing_root: Root           
+        ) returns (s: BLSSignature)
+        requires signing_root == compute_randao_reveal_signing_root(epoch * SLOTS_PER_EPOCH)
+    }
+
+    // NOTE: All methods in this trait MUST be implemented thread-safe.
+    trait {:autocontracts} SlashingDB<SlashingDBType(==)>
+    {
+        ghost var slashingDBRecords: imaptotal<BLSPubkey, set<SlashingDBType>>;
+
+        method add_record(new_record: SlashingDBType, pubkey: BLSPubkey)
+        ensures slashingDBRecords == old(slashingDBRecords)[pubkey := old(slashingDBRecords)[pubkey] + {new_record}]
+
+        method get_records(pubkey: BLSPubkey) returns (records: set<SlashingDBType>)
+        ensures records == this.slashingDBRecords[pubkey]
+    }   
+
+    // trait {:autocontracts} BlockSlashingDB
+    // {
+    //     ghost var blocks: imaptotal<BLSPubkey, set<SlashingDBBlock>>
+
+    //     method add_proposal(block: SlashingDBBlock, pubkey: BLSPubkey)
+    //     ensures blocks == old(blocks)[pubkey := old(blocks)[pubkey] + {block}]
+
+    //     method get_proposals(pubkey: BLSPubkey) returns (blocks: set<SlashingDBBlock>)
+    //     ensures blocks == this.blocks[pubkey]
+    // }    
+}
+
